\input article

\parindent=5mm

\SetFontSizesX

\section{One dimension}

For a distribution $h(x)$ let us define
\eqref{\eqnarray{
\hbox{mean } \mu &= \int \d x\, h(x)\, x\cr
\hbox{variance } \si^2 &= \int \d x\, h(x)\, (x-\mu)^2\cr
\hbox{standard deviation } \si &= \sqrt{\si^2}\cr
\hbox{fourth central moment } E_4 &= \int \d x\, h(x)\, (x-\mu)^4\ .\cr
}}{mu si}

The {\bf mean estimator}
\eqref{\hat\mu = {1\over N}\sum_i^N x_i}{hat mu}
is
\eqref{\eqnarray{
\hbox{unbiased} &: E[\hat\mu] = \mu\cr
\hbox{consistent} &: \hat\mu \mathop{\longrightarrow}\limits^{N\to \infty} \mu\cr
}}{hat mu prop}
and its variation
\eqref{V[\hat\mu] = {\si^2\over N}\ .}{V hat mu}

The {\bf variance estimator}
\eqref{\widehat{\si^2} = {1\over N - 1} \sum_i^N \left( x_i - \hat\mu \right)^2 = {1\over N-1} \left[ \sum x_i^2 - {1\over N} \left(\sum x_i\right)^2 \right]}{hat si}
is also unbiased. The estimator has variance
\eqref{V[\widehat{\si^2}] = {1\over N} \left( E_4 - {N-3\over N-1} \si^4 \right)\ .}{V hat si}

The {\bf $E_4$ estimator}
\eqref{
	\widehat{E_4} = {1\over N-1}\sum_i^N (x_i - \hat\mu)^4 = 
	{1\over N-1} \left( \sum x^4 - 4\hat\mu\sum x^3 + 6\hat\mu^2\sum x^2 - 4\hat\mu^3\sum x + \hat\mu^4 \sum 1 \right )\ .
}{hat E 4}

The {\bf standard-deviation estimator}
\eqref{\hat\si = \sqrt{\widehat{\si^2}}}{std dev estim}
has a variance of
\eqref{V[\hat\si] = {V[\widehat{\si^2}]\over 4\widehat{\si^2}}\ .}{std dev estim var}
For Gaussian distribution it reduces to
\eqref{V[\hat\si] = {\si^2\over 2N}\ .}{std dev estim var}

To {\bf summarize}, the mean and standard deviation of sample (value $\pm$ standard deviation of the estimator) can be estimated as follows:
\eqref{\eqnarray{
\hbox{mean} &: \hat\mu \pm \sqrt{\widehat{\si^2}\over N}\cr
\hbox{standard deviation} &: \sqrt{\widehat{\si^2}} \pm \sqrt{A\over \widehat{\si^2}}\ ,\qquad A = {1\over N} \left[ \widehat{E_4} - {N-3\over N-1} \left(\widehat{\si^2}\right)^2 \right]\cr
}}{summary}


\vfil
\eject


\section{Two dimensions}

For a distribution $h(x, y)$ let us define
\eqref{\eqnarray{
\hbox{mean in $x$: }\ \mu_x &= \int\!\! \int \d x\, \d y\ h(x, y)\, x\cr
\hbox{mean in $y$: } \mu_y &= \int\!\! \int \d x\, \d y\ h(x, y)\, y\cr
\hbox{covariance between $x$ and $y$: }\ C_{xy} &= \int\!\! \int \d x\, \d y\ h(x, y)\, (x - \mu_x) (y - \mu_y)\cr
}}{two mu si}

The {\bf mean estimators}
\eqref{\widehat{\mu_x} = {1\over N}\sum_i^N x_i\ ,\qquad \widehat{\mu_y} = {1\over N}\sum_i^N y_i}{hat mu x y}
are unbiased and consistent.

This {\bf covariance estimator}
\eqref{\widehat{C_{xy}}
	= {1\over N-1} \sum\limits_i^N (x_i - \widehat{\mu_x})\, (y_i - \widehat{\mu_y})
	= {1\over N-1} \left[ \sum x_i y_i - {1\over N} (\sum x_i)\, (\sum y_i) \right]
}{covar estim}
is unbiased.

\bye
